Factor wordlist_from_memory out of Keccak proofs and generalize
This moves the construct "wordlist_from_memory" that is used in the
Keccak specifications back into the general background theory,
currently in common/bignum.ml. It now has a generalized word type
instead of being restricted to 64 bits, and hence can be used in
other contexts, though the nicest versions of some theorems hold
when the word size is a multiple of 8 or more generally the total
number of bits in the region is a multiple of 8. In support of
the general background, "wordlist_of_num" is also added, a natural
inverse to "num_of_wordlist".

arm/proofs/mlkem_keccak2_f1600_alt.ml
@@ -229,32 +229,6 @@ let mlkem_keccak2_f1600_alt_mc = define_assert_from_elf
 let MLKEM_KECCAK2_F1600_ALT_EXEC = ARM_MK_EXEC_RULE mlkem_keccak2_f1600_alt_mc;;
 
 (* ------------------------------------------------------------------------- *)
-(* Convenient constructs to state and prove correctness. Should possibly     *)
-(* introduce a full state component for word lists eventually.               *)
-(* ------------------------------------------------------------------------- *)
-
-let wordlist_from_memory = define
- `wordlist_from_memory(a,0) s = [] /\
-  wordlist_from_memory(a,SUC n) s =
-  APPEND (wordlist_from_memory(a,n) s)
-         [read (memory :> bytes64(word_add a (word(8 * n)))) s]`;;
-
-(*** This is very naive and should be done more efficiently ***)
-
-let WORDLIST_FROM_MEMORY_CONV =
-  let uconv =
-    (LAND_CONV(RAND_CONV num_CONV) THENC
-     GEN_REWRITE_CONV I [CONJUNCT2 wordlist_from_memory]) ORELSEC
-     GEN_REWRITE_CONV I [CONJUNCT1 wordlist_from_memory] in
-  let conv =
-    TOP_DEPTH_CONV uconv THENC
-    ONCE_DEPTH_CONV NUM_MULT_CONV THENC
-    GEN_REWRITE_CONV ONCE_DEPTH_CONV [WORD_ADD_0] THENC
-    GEN_REWRITE_CONV TOP_DEPTH_CONV [APPEND]
-  and filt = can (term_match [] `wordlist_from_memory(a,NUMERAL n) s`) in
-  conv o check filt;;
-
-(* ------------------------------------------------------------------------- *)
 (* Correctness proof                                                         *)
 (* ------------------------------------------------------------------------- *)
 
@@ -310,7 +284,7 @@ let MLKEM_KECCAK2_F1600_ALT_CORRECT = prove
     (*** Initial holding of the invariant ***)
 
     REWRITE_TAC[round_constants; CONS_11; GSYM CONJ_ASSOC;
-                WORDLIST_FROM_MEMORY_CONV `wordlist_from_memory(rc,24) s`] THEN
+     WORDLIST_FROM_MEMORY_CONV `wordlist_from_memory(rc,24) s:int64 list`] THEN
     ENSURES_INIT_TAC "s0" THEN
     BIGNUM_DIGITIZE_TAC "A_" `read (memory :> bytes (a,8 * 50)) s0` THEN
     REPEAT(FIRST_X_ASSUM
@@ -331,7 +305,7 @@ let MLKEM_KECCAK2_F1600_ALT_CORRECT = prove
 
     X_GEN_TAC `i:num` THEN STRIP_TAC THEN VAL_INT64_TAC `i:num` THEN
     REWRITE_TAC[round_constants; CONS_11; GSYM CONJ_ASSOC;
-                WORDLIST_FROM_MEMORY_CONV `wordlist_from_memory(rc,24) s`] THEN
+     WORDLIST_FROM_MEMORY_CONV `wordlist_from_memory(rc,24) s:int64 list`] THEN
     MP_TAC(ISPECL [`A:int64 list`; `i:num`] LENGTH_KECCAK) THEN
     MP_TAC(ISPECL [`A':int64 list`; `i:num`] LENGTH_KECCAK) THEN
     ASM_REWRITE_TAC[IMP_IMP] THEN REWRITE_TAC[LENGTH_EQ_25] THEN
@@ -359,13 +333,13 @@ let MLKEM_KECCAK2_F1600_ALT_CORRECT = prove
 
     X_GEN_TAC `i:num` THEN STRIP_TAC THEN
     REWRITE_TAC[round_constants; CONS_11; GSYM CONJ_ASSOC;
-    WORDLIST_FROM_MEMORY_CONV `wordlist_from_memory(rc,24) s`] THEN
+     WORDLIST_FROM_MEMORY_CONV `wordlist_from_memory(rc,24) s:int64 list`] THEN
     ARM_SIM_TAC MLKEM_KECCAK2_F1600_ALT_EXEC [1] THEN
     VAL_INT64_TAC `i:num` THEN
     ASM_REWRITE_TAC[] THEN CONV_TAC(DEPTH_CONV WORD_NUM_RED_CONV) THEN
     ASM_SIMP_TAC[LT_IMP_NE];
 
-    (*** The tail of deferred rotations and writeback ***)
+    (*** The writeback tail ***)
 
     MP_TAC(ISPECL [`A:int64 list`; `24`] LENGTH_KECCAK) THEN
     MP_TAC(ISPECL [`A':int64 list`; `24`] LENGTH_KECCAK) THEN
